feat: finish proof

src/Std/Tactic/BVDecide/Bitblast/BVExpr/Circuit/Impl/Operations/Sdiv.lean
@@ -22,6 +22,61 @@ namespace bitblast
 
 variable [Hashable α] [DecidableEq α]
 
+namespace blastSdiv
+
+structure SignBranchInput (aig : AIG α) (len : Nat) where
+  w : Nat
+  lhs : AIG.RefVec aig w
+  rhs : AIG.RefVec aig w
+  lposRpos : AIG.RefVec aig len
+  lposRneg : AIG.RefVec aig len
+  lnegRpos : AIG.RefVec aig len
+  lnegRneg : AIG.RefVec aig len
+  hnezero : w ≠ 0
+
+def signBranch (aig : AIG α) (input : SignBranchInput aig len) : AIG.RefVecEntry α len :=
+ let ⟨w, lhs, rhs, lposRpos, lposRneg, lnegRpos, lnegRneg, hnezero⟩ := input
+ let res := AIG.RefVec.ite aig ⟨rhs.get (w - 1) (by omega), lposRneg, lposRpos⟩
+ let aig := res.aig
+ let lposHalf := res.vec
+ have := AIG.LawfulVecOperator.le_size (f := AIG.RefVec.ite) ..
+ let lhs := lhs.cast this
+ let rhs := rhs.cast this
+ let lnegRneg := lnegRneg.cast this
+ let lnegRpos := lnegRpos.cast this
+
+ let res := AIG.RefVec.ite aig ⟨rhs.get (w - 1) (by omega), lnegRneg, lnegRpos⟩
+ let aig := res.aig
+ let lnegHalf := res.vec
+ have := AIG.LawfulVecOperator.le_size (f := AIG.RefVec.ite) ..
+ let lhs := lhs.cast this
+ let lposHalf := lposHalf.cast this
+
+ AIG.RefVec.ite aig ⟨lhs.get (w - 1) (by omega), lnegHalf, lposHalf⟩
+
+instance : AIG.LawfulVecOperator α SignBranchInput signBranch where
+  le_size := by
+    intros
+    unfold signBranch
+    dsimp only
+    apply AIG.LawfulVecOperator.le_size_of_le_aig_size (f := AIG.RefVec.ite)
+    apply AIG.LawfulVecOperator.le_size_of_le_aig_size (f := AIG.RefVec.ite)
+    apply AIG.LawfulVecOperator.le_size (f := AIG.RefVec.ite)
+  decl_eq := by
+    intros
+    unfold signBranch
+    dsimp only
+    rw [AIG.LawfulVecOperator.decl_eq (f := AIG.RefVec.ite)]
+    rw [AIG.LawfulVecOperator.decl_eq (f := AIG.RefVec.ite)]
+    rw [AIG.LawfulVecOperator.decl_eq (f := AIG.RefVec.ite)]
+    · apply AIG.LawfulVecOperator.lt_size_of_lt_aig_size (f := AIG.RefVec.ite)
+      assumption
+    · apply AIG.LawfulVecOperator.lt_size_of_lt_aig_size (f := AIG.RefVec.ite)
+      apply AIG.LawfulVecOperator.lt_size_of_lt_aig_size (f := AIG.RefVec.ite)
+      assumption
+
+end blastSdiv
+
 def blastSdiv (aig : AIG α) (input : AIG.BinaryRefVec aig w) : AIG.RefVecEntry α w :=
   if h : w = 0 then
     ⟨aig, h ▸ AIG.RefVec.empty⟩
@@ -91,27 +146,83 @@ def blastSdiv (aig : AIG α) (input : AIG.BinaryRefVec aig w) : AIG.RefVecEntry 
     let lposRneg := lposRneg.cast this
     let lnegRpos := lnegRpos.cast this
 
-    let res := AIG.RefVec.ite aig ⟨rhs.get (w - 1) (by omega), lposRneg, lposRpos⟩
-    let aig := res.aig
-    let lposHalf := res.vec
-    have := AIG.LawfulVecOperator.le_size (f := AIG.RefVec.ite) ..
-    let lhs := lhs.cast this
-    let rhs := rhs.cast this
-    let lnegRneg := lnegRneg.cast this
-    let lnegRpos := lnegRpos.cast this
-
-    let res := AIG.RefVec.ite aig ⟨rhs.get (w - 1) (by omega), lnegRneg, lnegRpos⟩
-    let aig := res.aig
-    let lnegHalf := res.vec
-    have := AIG.LawfulVecOperator.le_size (f := AIG.RefVec.ite) ..
-    let lhs := lhs.cast this
-    let lposHalf := lposHalf.cast this
-
-    AIG.RefVec.ite aig ⟨lhs.get (w - 1) (by omega), lnegHalf, lposHalf⟩
+    blastSdiv.signBranch aig ⟨w, lhs, rhs, lposRpos, lposRneg, lnegRpos, lnegRneg, h⟩
 
 instance : AIG.LawfulVecOperator α AIG.BinaryRefVec blastSdiv where
-  le_size := sorry
-  decl_eq := sorry
+  le_size := by
+    intros
+    unfold blastSdiv
+    dsimp only
+    split
+    · simp
+    · apply AIG.LawfulVecOperator.le_size_of_le_aig_size (f := blastSdiv.signBranch)
+      apply AIG.LawfulVecOperator.le_size_of_le_aig_size (f := blastUdiv)
+      apply AIG.LawfulVecOperator.le_size_of_le_aig_size (f := blastNeg)
+      apply AIG.LawfulVecOperator.le_size_of_le_aig_size (f := blastUdiv)
+      apply AIG.LawfulVecOperator.le_size_of_le_aig_size (f := blastNeg)
+      apply AIG.LawfulVecOperator.le_size_of_le_aig_size (f := blastUdiv)
+      apply AIG.LawfulVecOperator.le_size_of_le_aig_size (f := blastUdiv)
+      apply AIG.LawfulVecOperator.le_size_of_le_aig_size (f := blastNeg)
+      apply AIG.LawfulVecOperator.le_size (f := blastNeg)
+  decl_eq := by
+    intros
+    unfold blastSdiv
+    dsimp only
+    split
+    · simp
+    · rw [AIG.LawfulVecOperator.decl_eq (f := blastSdiv.signBranch)]
+      rw [AIG.LawfulVecOperator.decl_eq (f := blastUdiv)]
+      rw [AIG.LawfulVecOperator.decl_eq (f := blastNeg)]
+      rw [AIG.LawfulVecOperator.decl_eq (f := blastUdiv)]
+      rw [AIG.LawfulVecOperator.decl_eq (f := blastNeg)]
+      rw [AIG.LawfulVecOperator.decl_eq (f := blastUdiv)]
+      rw [AIG.LawfulVecOperator.decl_eq (f := blastUdiv)]
+      rw [AIG.LawfulVecOperator.decl_eq (f := blastNeg)]
+      rw [AIG.LawfulVecOperator.decl_eq (f := blastNeg)]
+      · apply AIG.LawfulVecOperator.lt_size_of_lt_aig_size (f := blastNeg)
+        assumption
+      · apply AIG.LawfulVecOperator.lt_size_of_lt_aig_size (f := blastNeg)
+        apply AIG.LawfulVecOperator.lt_size_of_lt_aig_size (f := blastNeg)
+        assumption
+      · apply AIG.LawfulVecOperator.lt_size_of_lt_aig_size (f := blastUdiv)
+        apply AIG.LawfulVecOperator.lt_size_of_lt_aig_size (f := blastNeg)
+        apply AIG.LawfulVecOperator.lt_size_of_lt_aig_size (f := blastNeg)
+        assumption
+      · apply AIG.LawfulVecOperator.lt_size_of_lt_aig_size (f := blastUdiv)
+        apply AIG.LawfulVecOperator.lt_size_of_lt_aig_size (f := blastUdiv)
+        apply AIG.LawfulVecOperator.lt_size_of_lt_aig_size (f := blastNeg)
+        apply AIG.LawfulVecOperator.lt_size_of_lt_aig_size (f := blastNeg)
+        assumption
+      · apply AIG.LawfulVecOperator.lt_size_of_lt_aig_size (f := blastNeg)
+        apply AIG.LawfulVecOperator.lt_size_of_lt_aig_size (f := blastUdiv)
+        apply AIG.LawfulVecOperator.lt_size_of_lt_aig_size (f := blastUdiv)
+        apply AIG.LawfulVecOperator.lt_size_of_lt_aig_size (f := blastNeg)
+        apply AIG.LawfulVecOperator.lt_size_of_lt_aig_size (f := blastNeg)
+        assumption
+      · apply AIG.LawfulVecOperator.lt_size_of_lt_aig_size (f := blastUdiv)
+        apply AIG.LawfulVecOperator.lt_size_of_lt_aig_size (f := blastNeg)
+        apply AIG.LawfulVecOperator.lt_size_of_lt_aig_size (f := blastUdiv)
+        apply AIG.LawfulVecOperator.lt_size_of_lt_aig_size (f := blastUdiv)
+        apply AIG.LawfulVecOperator.lt_size_of_lt_aig_size (f := blastNeg)
+        apply AIG.LawfulVecOperator.lt_size_of_lt_aig_size (f := blastNeg)
+        assumption
+      · apply AIG.LawfulVecOperator.lt_size_of_lt_aig_size (f := blastNeg)
+        apply AIG.LawfulVecOperator.lt_size_of_lt_aig_size (f := blastUdiv)
+        apply AIG.LawfulVecOperator.lt_size_of_lt_aig_size (f := blastNeg)
+        apply AIG.LawfulVecOperator.lt_size_of_lt_aig_size (f := blastUdiv)
+        apply AIG.LawfulVecOperator.lt_size_of_lt_aig_size (f := blastUdiv)
+        apply AIG.LawfulVecOperator.lt_size_of_lt_aig_size (f := blastNeg)
+        apply AIG.LawfulVecOperator.lt_size_of_lt_aig_size (f := blastNeg)
+        assumption
+      · apply AIG.LawfulVecOperator.lt_size_of_lt_aig_size (f := blastUdiv)
+        apply AIG.LawfulVecOperator.lt_size_of_lt_aig_size (f := blastNeg)
+        apply AIG.LawfulVecOperator.lt_size_of_lt_aig_size (f := blastUdiv)
+        apply AIG.LawfulVecOperator.lt_size_of_lt_aig_size (f := blastNeg)
+        apply AIG.LawfulVecOperator.lt_size_of_lt_aig_size (f := blastUdiv)
+        apply AIG.LawfulVecOperator.lt_size_of_lt_aig_size (f := blastUdiv)
+        apply AIG.LawfulVecOperator.lt_size_of_lt_aig_size (f := blastNeg)
+        apply AIG.LawfulVecOperator.lt_size_of_lt_aig_size (f := blastNeg)
+        assumption
 
 end bitblast
 end BVExpr
