src/Std/Tactic/BVDecide/Bitblast/BVExpr/Circuit/Lemmas/Operations/Sdiv.lean
@@ -23,21 +23,61 @@ namespace bitblast
 
 variable [Hashable α] [DecidableEq α]
 
-private theorem sdiv_of_pos_of_pos {lhs rhs : BitVec w} (h1 : lhs.msb = false) (h2 : rhs.msb = false) :
-    lhs.sdiv rhs = lhs / rhs := by
-  simp [BitVec.sdiv_eq, h1, h2]
+namespace blastSdiv
 
-private theorem sdiv_of_pos_of_neg {lhs rhs : BitVec w} (h1 : lhs.msb = false) (h2 : rhs.msb = true) :
-    lhs.sdiv rhs = -(lhs / -rhs) := by
-  simp [BitVec.sdiv_eq, h1, h2]
+theorem denote_signBranch {aig : AIG α} (input : SignBranchInput aig len) (lhs rhs : BitVec input.w)
+    (lposRpos lposRneg lnegRpos lnegRneg : BitVec len)
+    (hleft : ∀ (idx : Nat) (hidx : idx < input.w), ⟦aig, input.lhs.get idx hidx, assign⟧ = lhs.getLsbD idx)
+    (hright : ∀ (idx : Nat) (hidx : idx < input.w), ⟦aig, input.rhs.get idx hidx, assign⟧ = rhs.getLsbD idx)
+    (hlprp : ∀ (idx : Nat) (hidx : idx < len), ⟦aig, input.lposRpos.get idx hidx, assign⟧ = lposRpos.getLsbD idx)
+    (hlprn : ∀ (idx : Nat) (hidx : idx < len), ⟦aig, input.lposRneg.get idx hidx, assign⟧ = lposRneg.getLsbD idx)
+    (hlnrp : ∀ (idx : Nat) (hidx : idx < len), ⟦aig, input.lnegRpos.get idx hidx, assign⟧ = lnegRpos.getLsbD idx)
+    (hlnrn : ∀ (idx : Nat) (hidx : idx < len), ⟦aig, input.lnegRneg.get idx hidx, assign⟧ = lnegRneg.getLsbD idx) :
+  ∀ (idx : Nat) (hidx : idx < len),
+    ⟦(signBranch aig input).aig, (signBranch aig input).vec.get idx hidx, assign⟧
+      =
+    (match lhs.msb, rhs.msb with
+    | false, false => lposRpos
+    | false, true => lposRneg
+    | true, false => lnegRpos
+    | true, true => lnegRneg).getLsbD idx
+    := by
+  intros
+  unfold signBranch
+  simp
+  split
+  · next h1 =>
+    rw [AIG.LawfulVecOperator.denote_mem_prefix, AIG.LawfulVecOperator.denote_mem_prefix] at h1
+    rw [hleft, ← BitVec.msb_eq_getLsbD_last] at h1
+    rw [h1]
+    split
+    · next h2 =>
+      rw [AIG.LawfulVecOperator.denote_mem_prefix] at h2
+      rw [hright, ← BitVec.msb_eq_getLsbD_last] at h2
+      rw [h2]
+      rw [AIG.LawfulVecOperator.denote_mem_prefix, hlnrn]
+    · next h2 =>
+      rw [AIG.LawfulVecOperator.denote_mem_prefix] at h2
+      rw [hright, ← BitVec.msb_eq_getLsbD_last, Bool.not_eq_true] at h2
+      rw [h2]
+      rw [AIG.LawfulVecOperator.denote_mem_prefix, hlnrp]
+  · next h1 =>
+    rw [AIG.LawfulVecOperator.denote_mem_prefix, AIG.LawfulVecOperator.denote_mem_prefix] at h1
+    rw [hleft, ← BitVec.msb_eq_getLsbD_last, Bool.not_eq_true] at h1
+    rw [h1]
+    rw [AIG.LawfulVecOperator.denote_mem_prefix]
+    rw [AIG.RefVec.denote_ite]
+    split
+    · next h2 =>
+      rw [hright, ← BitVec.msb_eq_getLsbD_last] at h2
+      rw [h2]
+      simp [hlprn]
+    · next h2 =>
+      rw [hright, ← BitVec.msb_eq_getLsbD_last, Bool.not_eq_true] at h2
+      rw [h2]
+      simp [hlprp]
 
-private theorem sdiv_of_neg_of_pos {lhs rhs : BitVec w} (h1 : lhs.msb = true) (h2 : rhs.msb = false) :
-    lhs.sdiv rhs = -(-lhs / rhs) := by
-  simp [BitVec.sdiv_eq, h1, h2]
-
-private theorem sdiv_of_neg_of_neg {lhs rhs : BitVec w} (h1 : lhs.msb = true) (h2 : rhs.msb = true) :
-    lhs.sdiv rhs = (-lhs) / (-rhs) := by
-  simp [BitVec.sdiv_eq, h1, h2]
+end blastSdiv
 
 theorem denote_blastSdiv (aig : AIG α) (lhs rhs : BitVec w) (assign : α → Bool)
       (input : BinaryRefVec aig w)
@@ -46,147 +86,114 @@ theorem denote_blastSdiv (aig : AIG α) (lhs rhs : BitVec w) (assign : α → Bo
       ∀ (idx : Nat) (hidx : idx < w),
         ⟦(blastSdiv aig input).aig, (blastSdiv aig input).vec.get idx hidx, assign⟧
           =
-        (BitVec.sdiv lhs rhs).getLsbD idx := by sorry
-/-
+        (BitVec.sdiv lhs rhs).getLsbD idx := by
   intros
   generalize hres : blastSdiv aig input = res
   unfold blastSdiv at hres
   split at hres
   · omega
-  · rw [← hres]
+  · dsimp only at hres
+    rw [← hres]
     clear hres
-    simp only [RefVec.denote_ite, RefVec.get_cast, Ref.cast_eq]
-    split
-    · next h1 =>
+    rw [blastSdiv.denote_signBranch
+        (lhs := lhs)
+        (rhs := rhs)
+        (lposRpos := lhs / rhs)
+        (lposRneg := -(lhs / (-rhs)))
+        (lnegRpos := -((-lhs) / rhs))
+        (lnegRneg := ((-lhs) / (-rhs)))
+      ]
+    · rw [BitVec.sdiv_eq]
+      rfl
+    · simp only [RefVec.get_cast, Ref.cast_eq]
+      intros
       rw [AIG.LawfulVecOperator.denote_mem_prefix, AIG.LawfulVecOperator.denote_mem_prefix,
-       AIG.LawfulVecOperator.denote_mem_prefix, AIG.LawfulVecOperator.denote_mem_prefix,
-       AIG.LawfulVecOperator.denote_mem_prefix, AIG.LawfulVecOperator.denote_mem_prefix,
-       AIG.LawfulVecOperator.denote_mem_prefix, AIG.LawfulVecOperator.denote_mem_prefix,
-       AIG.LawfulVecOperator.denote_mem_prefix, AIG.LawfulVecOperator.denote_mem_prefix] at h1
-      rw [hleft, ← BitVec.msb_eq_getLsbD_last ] at h1
-      split
-      · next h2 =>
-        rw [AIG.LawfulVecOperator.denote_mem_prefix, AIG.LawfulVecOperator.denote_mem_prefix,
-            AIG.LawfulVecOperator.denote_mem_prefix, AIG.LawfulVecOperator.denote_mem_prefix,
-            AIG.LawfulVecOperator.denote_mem_prefix, AIG.LawfulVecOperator.denote_mem_prefix,
-            AIG.LawfulVecOperator.denote_mem_prefix, AIG.LawfulVecOperator.denote_mem_prefix,
-            AIG.LawfulVecOperator.denote_mem_prefix] at h2
-        rw [hright, ← BitVec.msb_eq_getLsbD_last ] at h2
-        rw [AIG.LawfulVecOperator.denote_mem_prefix]
-        rw [denote_blastUdiv (lhs := -lhs) (rhs := -rhs)]
-        · rw [sdiv_of_neg_of_neg h1 h2]
-        · intros
-          rw [AIG.LawfulVecOperator.denote_mem_prefix, AIG.LawfulVecOperator.denote_mem_prefix,
-              AIG.LawfulVecOperator.denote_mem_prefix,
-              AIG.LawfulVecOperator.denote_mem_prefix,
-              AIG.LawfulVecOperator.denote_mem_prefix,
-              AIG.LawfulVecOperator.denote_mem_prefix,
-          ]
-          · simp only [RefVec.get_cast, Ref.cast_eq]
-            rw [denote_blastNeg]
-            exact hleft
-          · simp [Ref.hgate]
-        · intros
-          simp only [RefVec.get_cast, Ref.cast_eq]
-          rw [AIG.LawfulVecOperator.denote_mem_prefix, AIG.LawfulVecOperator.denote_mem_prefix,
-              AIG.LawfulVecOperator.denote_mem_prefix,
-              AIG.LawfulVecOperator.denote_mem_prefix,
-              AIG.LawfulVecOperator.denote_mem_prefix,
-          ]
-          rw [denote_blastNeg]
-          intros
-          simp only [RefVec.get_cast, Ref.cast_eq]
-          rw [AIG.LawfulVecOperator.denote_mem_prefix]
-          rw [hright]
-      · next h2 =>
-        rw [AIG.LawfulVecOperator.denote_mem_prefix, AIG.LawfulVecOperator.denote_mem_prefix,
-            AIG.LawfulVecOperator.denote_mem_prefix, AIG.LawfulVecOperator.denote_mem_prefix,
-            AIG.LawfulVecOperator.denote_mem_prefix, AIG.LawfulVecOperator.denote_mem_prefix,
-            AIG.LawfulVecOperator.denote_mem_prefix, AIG.LawfulVecOperator.denote_mem_prefix,
-            AIG.LawfulVecOperator.denote_mem_prefix] at h2
-        rw [hright, ← BitVec.msb_eq_getLsbD_last, Bool.not_eq_true] at h2
+        AIG.LawfulVecOperator.denote_mem_prefix, AIG.LawfulVecOperator.denote_mem_prefix,
+        AIG.LawfulVecOperator.denote_mem_prefix, AIG.LawfulVecOperator.denote_mem_prefix,
+        AIG.LawfulVecOperator.denote_mem_prefix, AIG.LawfulVecOperator.denote_mem_prefix]
+      rw [hleft]
+    · simp only [RefVec.get_cast, Ref.cast_eq]
+      intros
+      rw [AIG.LawfulVecOperator.denote_mem_prefix, AIG.LawfulVecOperator.denote_mem_prefix,
+        AIG.LawfulVecOperator.denote_mem_prefix, AIG.LawfulVecOperator.denote_mem_prefix,
+        AIG.LawfulVecOperator.denote_mem_prefix, AIG.LawfulVecOperator.denote_mem_prefix,
+        AIG.LawfulVecOperator.denote_mem_prefix, AIG.LawfulVecOperator.denote_mem_prefix]
+      rw [hright]
+    · simp only [RefVec.get_cast, Ref.cast_eq]
+      intros
+      rw [AIG.LawfulVecOperator.denote_mem_prefix, AIG.LawfulVecOperator.denote_mem_prefix,
+        AIG.LawfulVecOperator.denote_mem_prefix, AIG.LawfulVecOperator.denote_mem_prefix,
+        AIG.LawfulVecOperator.denote_mem_prefix]
+      rw [denote_blastUdiv (lhs := lhs) (rhs := rhs)]
+      · intros
         rw [AIG.LawfulVecOperator.denote_mem_prefix, AIG.LawfulVecOperator.denote_mem_prefix]
-        rw [denote_blastNeg (value := (-lhs) / rhs)]
-        · rw [sdiv_of_neg_of_pos h1 h2]
-        · intros
-          rw [denote_blastUdiv (lhs := -lhs) (rhs := rhs)]
-          · intros
-            rw [AIG.LawfulVecOperator.denote_mem_prefix, AIG.LawfulVecOperator.denote_mem_prefix,
-                AIG.LawfulVecOperator.denote_mem_prefix, AIG.LawfulVecOperator.denote_mem_prefix,
-            ]
-            simp only [RefVec.get_cast, Ref.cast_eq]
-            rw [denote_blastNeg (value := lhs)]
-            · exact hleft
-            · simp [Ref.hgate]
-          · intros
-            rw [AIG.LawfulVecOperator.denote_mem_prefix, AIG.LawfulVecOperator.denote_mem_prefix,
-                AIG.LawfulVecOperator.denote_mem_prefix, AIG.LawfulVecOperator.denote_mem_prefix,
-                AIG.LawfulVecOperator.denote_mem_prefix]
-            · simp [hright]
-            · simp [Ref.hgate]
-    · next h1 =>
-      rw [AIG.LawfulVecOperator.denote_mem_prefix, AIG.LawfulVecOperator.denote_mem_prefix,
-          AIG.LawfulVecOperator.denote_mem_prefix, AIG.LawfulVecOperator.denote_mem_prefix,
-          AIG.LawfulVecOperator.denote_mem_prefix, AIG.LawfulVecOperator.denote_mem_prefix,
-          AIG.LawfulVecOperator.denote_mem_prefix, AIG.LawfulVecOperator.denote_mem_prefix,
-          AIG.LawfulVecOperator.denote_mem_prefix, AIG.LawfulVecOperator.denote_mem_prefix] at h1
-      rw [hleft, ← BitVec.msb_eq_getLsbD_last, Bool.not_eq_true] at h1
-      rw [AIG.LawfulVecOperator.denote_mem_prefix (f := AIG.RefVec.ite)]
-      rw [AIG.RefVec.denote_ite]
-      split
-      · next h2 =>
-        rw [AIG.LawfulVecOperator.denote_mem_prefix, AIG.LawfulVecOperator.denote_mem_prefix,
-         AIG.LawfulVecOperator.denote_mem_prefix, AIG.LawfulVecOperator.denote_mem_prefix,
-         AIG.LawfulVecOperator.denote_mem_prefix, AIG.LawfulVecOperator.denote_mem_prefix,
-         AIG.LawfulVecOperator.denote_mem_prefix, AIG.LawfulVecOperator.denote_mem_prefix,
-        ] at h2
-        simp only [RefVec.get_cast, Ref.cast_eq] at h2
-        rw [hright, ← BitVec.msb_eq_getLsbD_last] at h2
-        rw [AIG.LawfulVecOperator.denote_mem_prefix, AIG.LawfulVecOperator.denote_mem_prefix,
-         AIG.LawfulVecOperator.denote_mem_prefix]
-        · simp only [RefVec.get_cast, Ref.cast_eq]
-          rw [denote_blastNeg (value := lhs / (-rhs))]
-          · rw [sdiv_of_pos_of_neg h1 h2]
-          · intros
-            rw [denote_blastUdiv (lhs := lhs) (rhs := -rhs)]
-            · intros
-              rw [AIG.LawfulVecOperator.denote_mem_prefix, AIG.LawfulVecOperator.denote_mem_prefix,
-                  AIG.LawfulVecOperator.denote_mem_prefix]
-              · simp [hleft]
-              · simp [Ref.hgate]
-            · intros
-              rw [AIG.LawfulVecOperator.denote_mem_prefix]
-              · simp only [RefVec.get_cast, Ref.cast_eq]
-                rw [denote_blastNeg (value := rhs)]
-                intros
-                rw [AIG.LawfulVecOperator.denote_mem_prefix]
-                · simp [hright]
-                · simp [Ref.hgate]
-              · simp [Ref.hgate]
+        · simp [hleft]
         · simp [Ref.hgate]
-      · next h2 =>
+      · intros
+        rw [AIG.LawfulVecOperator.denote_mem_prefix, AIG.LawfulVecOperator.denote_mem_prefix]
+        · simp [hright]
+        · simp [Ref.hgate]
+    · simp only [RefVec.get_cast, Ref.cast_eq]
+      intros
+      rw [AIG.LawfulVecOperator.denote_mem_prefix, AIG.LawfulVecOperator.denote_mem_prefix,
+        AIG.LawfulVecOperator.denote_mem_prefix]
+      rw [denote_blastNeg (value := lhs / (-rhs))]
+      intros
+      rw [denote_blastUdiv (lhs := lhs) (rhs := -rhs)]
+      · intros
         rw [AIG.LawfulVecOperator.denote_mem_prefix, AIG.LawfulVecOperator.denote_mem_prefix,
-         AIG.LawfulVecOperator.denote_mem_prefix, AIG.LawfulVecOperator.denote_mem_prefix,
-         AIG.LawfulVecOperator.denote_mem_prefix, AIG.LawfulVecOperator.denote_mem_prefix,
-         AIG.LawfulVecOperator.denote_mem_prefix, AIG.LawfulVecOperator.denote_mem_prefix,
-        ] at h2
-        simp only [RefVec.get_cast, Ref.cast_eq] at h2
-        rw [hright, ← BitVec.msb_eq_getLsbD_last, Bool.not_eq_true] at h2
+          AIG.LawfulVecOperator.denote_mem_prefix]
+        · simp [hleft]
+        · simp [Ref.hgate]
+      · intros
+        rw [AIG.LawfulVecOperator.denote_mem_prefix]
+        · simp only [RefVec.get_cast, Ref.cast_eq]
+          rw [denote_blastNeg (value := rhs)]
+          intros
+          rw [AIG.LawfulVecOperator.denote_mem_prefix]
+          · simp [hright]
+          · simp [Ref.hgate]
+        · simp [Ref.hgate]
+    · simp only [RefVec.get_cast, Ref.cast_eq]
+      intros
+      rw [AIG.LawfulVecOperator.denote_mem_prefix]
+      rw [denote_blastNeg (value := (-lhs) / rhs)]
+      intros
+      rw [denote_blastUdiv (lhs := -lhs) (rhs := rhs)]
+      · intros
         rw [AIG.LawfulVecOperator.denote_mem_prefix, AIG.LawfulVecOperator.denote_mem_prefix,
-         AIG.LawfulVecOperator.denote_mem_prefix, AIG.LawfulVecOperator.denote_mem_prefix,
-         AIG.LawfulVecOperator.denote_mem_prefix]
-        simp only [RefVec.get_cast, Ref.cast_eq]
-        · rw [denote_blastUdiv (lhs := lhs) (rhs := rhs)]
-          · rw [sdiv_of_pos_of_pos h1 h2]
-          · intros
-            rw [AIG.LawfulVecOperator.denote_mem_prefix, AIG.LawfulVecOperator.denote_mem_prefix]
-            · simp [hleft]
-            · simp [Ref.hgate]
-          · intros
-            rw [AIG.LawfulVecOperator.denote_mem_prefix, AIG.LawfulVecOperator.denote_mem_prefix]
-            · simp [hright]
-            · simp [Ref.hgate]
-        · simp [Ref.hgate]-/
+          AIG.LawfulVecOperator.denote_mem_prefix, AIG.LawfulVecOperator.denote_mem_prefix]
+        · simp only [RefVec.get_cast, Ref.cast_eq]
+          rw [denote_blastNeg (value := lhs)]
+          simp [hleft]
+        · simp [Ref.hgate]
+      · intros
+        rw [AIG.LawfulVecOperator.denote_mem_prefix, AIG.LawfulVecOperator.denote_mem_prefix,
+          AIG.LawfulVecOperator.denote_mem_prefix, AIG.LawfulVecOperator.denote_mem_prefix,
+          AIG.LawfulVecOperator.denote_mem_prefix]
+        · simp [hright]
+        · simp [Ref.hgate]
+    · simp only
+      intros
+      rw [denote_blastUdiv (lhs := -lhs) (rhs := - rhs)]
+      · intros
+        simp
+        rw [AIG.LawfulVecOperator.denote_mem_prefix, AIG.LawfulVecOperator.denote_mem_prefix,
+          AIG.LawfulVecOperator.denote_mem_prefix, AIG.LawfulVecOperator.denote_mem_prefix,
+          AIG.LawfulVecOperator.denote_mem_prefix, AIG.LawfulVecOperator.denote_mem_prefix]
+        rw [denote_blastNeg (value := lhs)]
+        simp [hleft]
+      · intros
+        simp
+        rw [AIG.LawfulVecOperator.denote_mem_prefix, AIG.LawfulVecOperator.denote_mem_prefix,
+          AIG.LawfulVecOperator.denote_mem_prefix, AIG.LawfulVecOperator.denote_mem_prefix,
+          AIG.LawfulVecOperator.denote_mem_prefix]
+        rw [denote_blastNeg (value := rhs)]
+        intros
+        rw [AIG.LawfulVecOperator.denote_mem_prefix]
+        · simp [hright]
+        · simp [Ref.hgate]
+
 
 end bitblast
 end BVExpr
